devel/Iron/Language/SimpleDelayed/SubstXX.v
@@ -2,104 +2,21 @@
 Require Export Iron.Language.SimpleDelayed.TypeX.
 
 
-(* Lookup the type of the given variable from a substitution. *)
-Fixpoint lookupSubstX (var: nat) (ss: substx) : option bind :=
- match ss with
- | nil                
- => None
-
- | BBind v t x :: rest
- => if beq_nat var v
-      then Some (BBind v t x)
-      else lookupSubstX var rest
- end.
-
-
 (* Apply an expression substitution to an expression. *)
-Fixpoint substXX (ss: substx) (xx: exp) : exp :=
+Fixpoint substXX (ss: @subst exp ty) (xx: exp) {struct xx} : exp  :=
  match xx with
  | XVar n
- => match lookupSubstX n ss with
+ => match lookupSubst n ss with
     | None                => xx
     | Some (BBind _ _ x)  => x
     end
 
  |  XAbs ss2 n t x
- => XAbs (ss >< map (substXB ss) ss2) n t x
+ => XAbs (ss >< mapExpOfSubst (substXX ss) ss2) n t x
 
  |  XApp x1 x2
  => XApp (substXX ss x1) (substXX ss x2)
- end
-
- with substXB (ss: substx) (bb: bind): bind :=
-       match bb with
-       | BBind n t x => BBind n t (substXX ss x)
-       end.
-
-
-Lemma map_stripB_substXB
- : forall bs1 bs2
- , map stripB (map (substXB bs1) bs2)
- = map stripB bs2.
-Proof.
- intros.
- induction bs2.
- simpl. auto.
- simpl. rewrite IHbs2.
- destruct a. simpl. auto.
-Qed.
-
-
-Lemma lookupSubstX_name 
- :  forall n1 n2 t e bs
- ,  lookupSubstX n1 bs = Some (BBind n2 t e)
- -> n1 = n2.
-Proof.
- intros.
- induction bs.
- - simpl in *. nope.
- - simpl in *. destruct a.
-   remember (n1 =? n) as X. destruct X.
-   + inverts H. eapply beq_nat_true. firstorder.
-   + firstorder.
-Qed.
-
-
-Lemma lookup_env_subst_none
- :  forall n te bs t
- ,  lookupEnv n (te >< map stripB bs) = Some t
- -> lookupSubstX n bs                 = None
- -> lookupEnv n te = Some t.
-Proof.
- intros.
- induction bs.
- - simpl in *. nope.
- - simpl in *. destruct a. simpl in H.
-   remember (n =? n0) as X. destruct X.
-   + inverts H.
-     nope.
-   + eapply IHbs. 
-     * auto. 
-     * assumption.
-Qed.
-
-
-Lemma lookup_env_subst_some
- :  forall n te bs e t t0
- ,  Forall (TypeB te) bs
- -> lookupEnv    n (te >< map stripB bs) = Some t
- -> lookupSubstX n bs                    = Some (BBind n t0 e)
- -> TypeX te e t.
-Proof.
- intros. gen n te e t t0.
- induction bs; intros.
- - simpl in *. nope.
- - simpl in *. destruct a. simpl in *.
-   remember (n =? n0) as X. destruct X.
-   + inverts H0. inverts H1.
-     inverts H.  inverts H2. assumption.
-   + inverts H; eauto.
-Qed.
+ end.
 
 
 (* Substitution of expressions in expressions preserves typing.
@@ -110,28 +27,28 @@ Qed.
    place at top level. 
 *)
 Lemma subst_exp_exp
- :  forall te bs x t
- ,  TypeX  (te >< map stripB bs) x t
- -> Forall (TypeB te) bs
- -> TypeX  te (substXX bs x) t.
+ :  forall te ss x t
+ ,  TypeX  (te >< stripS ss) x t
+ -> ForallSubstXT (TypeX te) ss
+ -> TypeX  te (substXX ss x) t.
 Proof.
- intros. gen te bs t.
- induction x using exp_mutind with
-  (PB := fun b => forall te bs
-      ,  TypeB (te >< map stripB bs) b
-      -> Forall (TypeB te) bs
-      -> TypeB te (substXB bs b))
-   ; intros; simpl in *; inverts_type.
+ intros. gen te ss t.
+ induction x using exp_iind;
+  intros; simpl in *; inverts_type.
 
  - Case "XVar".
-   remember (lookupSubstX n bs) as X.
-   destruct X.
+   remember (lookupSubst n ss) as o.
+   symmetry in Heqo.
+   destruct o.
 
    + SCase "variable matches".
      destruct b.
-     symmetry in HeqX.
-     eapply (lookup_env_subst_some n te bs e t t0) in H3; eauto.
-     lets D: lookupSubstX_name HeqX. inverts D. assumption.
+     eapply lookup_env_subst_some; eauto.
+
+     assert (n = n0) as HN.
+     eapply (@lookupSubst_name exp ty); eauto.
+     rewrite HN in *.
+     eauto.
 
    + SCase "variable does not match.".
      eapply TxVar.
@@ -139,22 +56,31 @@ Proof.
 
  - Case "XLam".
    eapply TxLam.
-   + eapply Forall_app; auto.
-     * eapply (Forall_insts te)  in H.
-       eapply (Forall_insts bs0) in H.
-       eapply (Forall_impls 
-               (fun b => TypeB (te >< map stripB bs0) b)) in H; auto.
-       eapply (Forall_impl_inner (Forall (TypeB te) bs0)) in H; auto.
+   + eapply ForallSubstXT_app; auto.
 
-   + rewrite map_app.
-     rewrite map_stripB_substXB.
+     eapply (Forall_inst te)  in H.
+     eapply (Forall_inst ss0) in H.
+     eapply (Forall_mp_const) in H; auto.
+
+     eapply (Forall_map 
+              (  fun xx => forall t
+              ,  TypeX (te >< stripS ss0) xx t
+              -> TypeX te (substXX ss0 xx) t)) in H.
+
+     eapply Forall_Forall2_right  in H.
+     eapply ForallSubstXT_fold    in H.
+
+     eapply ForallSubstXT_mapExpOfSubst.
+     eapply ForallSubstXT_mp; eauto.
+
+   + unfold stripS.
+     rewrite map_app.
+     rewrite stripS_fold.
+     rewrite stripS_mapExpOfSubst.
      rewrite <- app_assoc.
      assumption.
 
  - Case "XApp".
    eapply TxApp; eauto.
-
- - Case "BBind".
-   eapply TsSig; eauto.
 Qed.
 
