devel/Iron/Language/SimpleDelayed/TypeX.v
@@ -2,39 +2,27 @@
 Require Export Iron.Language.SimpleDelayed.Exp.
 
 
-Fixpoint stripB (b: bind): sig :=
- match b with
- | BBind n t _ => SSig n t
- end.
-
-
+(*******************************************************************)
 (* Typing judgement assigns a type to an expression. *)
 Inductive TypeX : tyenv -> exp -> ty -> Prop :=
  | TxVar 
-   :  forall te n t
-   ,  lookupEnv n te = Some t
-   -> TypeX te (XVar n) t
+   :  forall te v t
+   ,  lookupEnv v te = Some t
+   -> TypeX te (XVar v) t
 
  | TxLam
-   :  forall te bs n1 t1 x2 t2
-   ,  Forall (TypeB te) bs
-   -> TypeX (te >< map stripB bs :> SSig n1 t1) x2 t2
-   -> TypeX te (XAbs bs n1 t1 x2) (TFun t1 t2)
+   :  forall te ss v1 t1 x2 t2
+   ,  ForallSubstXT (TypeX te) ss
+   -> TypeX (te >< stripS ss :> SSig v1 t1) x2 t2
+   -> TypeX te (XAbs ss v1 t1 x2) (TFun t1 t2)
 
  | TxApp
    :  forall te x1 x2 t1 t2
    ,  TypeX te x1 (TFun t1 t2)
    -> TypeX te x2 t1
-   -> TypeX te (XApp x1 x2) t2
-
- with TypeB : tyenv -> bind -> Prop :=
- | TsSig
-   :  forall te n t x
-   ,  TypeX te x t
-   -> TypeB te (BBind n t x).
+   -> TypeX te (XApp x1 x2) t2.
 
 Hint Constructors TypeX.
-Hint Constructors TypeB.
 
 
 (* Invert all hypothesis that are compound typing statements. *)
@@ -44,7 +32,6 @@ Ltac inverts_type :=
    | [ H: TypeX _ (XVar _) _       |- _ ] => inverts H
    | [ H: TypeX _ (XAbs _ _ _ _) _ |- _ ] => inverts H
    | [ H: TypeX _ (XApp _ _) _     |- _ ] => inverts H
-   | [ H: TypeB _ (BBind _ _ _)    |- _ ] => inverts H
    end).
 
 
@@ -53,13 +40,12 @@ Definition Closed (xx: exp) : Prop :=
  exists t, TypeX nil xx t.
 
 
-
 (*******************************************************************)
 (* Forms of terms lemma. *)
 Lemma done_lam 
  :  forall x t1 t2
  ,  TypeX nil x (TFun t1 t2)
- -> Done x
+ -> Done   x
  -> isXAbs x.
 Proof.
  intros. gen t1 t2.
@@ -68,7 +54,7 @@ Proof.
  - Case "XVar".
    nope.
 
- - Case "XLam".
+ - Case "XAbs".
    nope.
 
  - Case "XApp".
@@ -79,7 +65,7 @@ Proof.
      * nope.
 
      * rip.
-       assert (Value (XAbs l n t x1)); auto.
+       assert (Value (XAbs ss v t x1)); auto.
        nope.
 
      * inverts_type.
