devel/Iron/Language/SimpleDelayed/Base.v
@@ -1,7 +1,15 @@
 
-Require Export Iron.Data.List.
-Require Export Iron.Tactics.Case.
-Require Export Iron.Tactics.LibTactics.
+Require Export LocalLibTactics.
+Require Export LocalLibTacticsCase.
+Require Export LocalLibDataLists.
+
+
+(********************************************************************)
+(* Override the default notation for lists to be right biased.
+   We're only using lists for environments and substitutions, 
+   where the right biased order is more natural. *)
+Notation "xs :> x"  := (x :: xs)   (at level 61, left associativity).
+Notation "xs >< ys" := (app ys xs) (at level 60, right associativity).
 
 
 (********************************************************************)
