devel/Iron/Language/SimpleDelayed/LocalLibDataLists.v
@@ -1,0 +1,133 @@
+
+Require Export Coq.Lists.List.
+Require Export LocalLibTactics.
+
+
+(********************************************************************)
+(* Forall Lemmas *)
+
+Lemma Forall_inst
+ :  forall {A B} a' xs (P: A -> B -> Prop)
+ ,  Forall (fun x => forall a, P a x) xs
+ -> Forall (fun x => P a' x) xs.
+Proof.
+ intros.
+ induction xs.
+ - auto.
+ - eapply Forall_cons.
+   + inverts H. eapply H2.
+   + inverts H. eapply IHxs. assumption.
+Qed.
+
+
+Lemma Forall_mp
+ :  forall {A} (P Q: A -> Prop)  xs
+ ,  Forall (fun x => P x -> Q x) xs
+ -> Forall (fun x => P x)        xs
+ -> Forall (fun x => Q x)        xs.
+Proof.
+ intros.
+ induction xs.
+ - auto.
+ - eapply Forall_cons.
+   + inverts H. inverts H0. auto.
+   + inverts H. inverts H0. auto.
+Qed. 
+
+
+Lemma Forall_mp_const 
+ :  forall {A} P (Q: A -> Prop)  xs
+ ,  P
+ -> Forall (fun x => P -> Q x) xs
+ -> Forall (fun x => Q x)      xs.
+Proof.
+ intros.
+ induction H.
+ - auto.
+ - apply Forall_cons.
+   + auto.
+   + auto.
+Qed.
+
+
+Lemma Forall_map
+ :  forall {A B}
+    (P: B -> Prop) (f: A -> B) (xs: list A)
+ ,  Forall (fun x => P (f x)) xs
+ -> Forall P (map f xs).
+Proof.
+ intros. induction xs.
+  apply Forall_nil.
+  inverts H. simpl. intuition.
+Qed.
+
+
+
+(********************************************************************)
+(* Forall2 Lemmas *)
+
+Lemma Forall2_mp
+ :  forall {A B} (P Q: A -> B -> Prop)  aa bb
+ ,  Forall2 (fun a b => P a b -> Q a b) aa bb
+ -> Forall2 (fun a b => P a b)          aa bb
+ -> Forall2 (fun a b => Q a b)          aa bb.
+Proof.
+ intros.
+ induction H0.
+ - auto.
+ - inverts H.
+   apply Forall2_cons; auto.
+Qed.
+
+
+Lemma Forall2_map
+ :  forall {A B C D}
+    (P:  B -> D -> Prop) (f:  A -> B) (g:  C -> D) 
+    (xs: list A) (ys: list C)
+ ,  Forall2 (fun x y => P (f x) (g y)) xs ys
+ -> Forall2 P (map f xs) (map g ys).
+Proof.
+ intros.
+ induction H.
+ - simpl. auto.
+ - simpl. apply Forall2_cons; auto. 
+Qed.
+
+
+Lemma Forall2_map'
+ :  forall {A B C D}
+    (P: B -> D -> Prop) (f:  A -> B) (g:  C -> D)
+    (xs: list A) (ys: list C)
+ ,  Forall2 P (map f xs) (map g ys)
+ -> Forall2 (fun x y => P (f x) (g y)) xs ys.
+Proof.
+ intros. gen ys.
+ induction xs; intros.
+  induction ys; intros.
+   auto.
+   inverts H.
+   destruct ys.
+    inverts H.
+    simpl in H.
+    inverts H. eauto.
+Qed.
+
+
+(********************************************************************)
+(* Convert Forall to Forall2 *)
+Lemma Forall_Forall2_right
+ :  forall  {A B C} 
+    (P: B -> C -> Prop) 
+    (f: A -> B) (g: A -> C) (aa: list A)
+ ,  Forall  (fun b => forall c, P b c) (map f aa)
+ -> Forall2 P (map f aa) (map g aa).
+Proof.
+ intros.
+ induction aa.
+ - simpl. auto.
+ - simpl in *.
+   inverts H.
+   apply Forall2_cons.
+   auto. auto.
+Qed.
+
