devel/Iron/Language/SimpleDelayed/Subst.v
@@ -1,0 +1,246 @@
+
+Require Export Coq.Strings.String.
+Require Export LocalLibTactics.
+Require Export LocalLibDataLists.
+
+
+(********************************************************************)
+(* Variables want to be named. *)
+Definition name := string.
+
+
+(********************************************************************)
+(* Type signatures *)
+Inductive  sig {A: Type}: Type :=
+ | SSig  : name -> A -> @sig A.
+
+
+(* An environment is a list of signatures. *)
+Definition env (A: Type) 
+ := list (@sig A).
+
+
+(* Lookup the type of the given variable from an environment. *)
+Fixpoint lookupEnv {T: Type} (var: string) (ee: env T) : option T :=
+ match ee with
+ | nil                
+ => None
+
+ | SSig v t :: rest
+ => match string_dec var v with
+    | left  _ => Some t
+    | right _ => lookupEnv var rest
+    end
+ end.
+
+
+(********************************************************************)
+(* Typed bindings. *)
+Inductive bind {X: Type} {T: Type}: Type :=
+ | BBind   : name -> T -> X -> @bind X T.
+Hint Constructors bind.
+
+
+(* Get the type component of a binding. *)
+Definition typeOfBind {X T} (b: @bind X T): T :=
+ match b with
+ | BBind _ t x => t
+ end.
+
+
+(* Get the expression component of a binding. *)
+Definition expOfBind  {X T} (b: @bind X T): X :=
+ match b with
+ | BBind _ _ x => x
+ end.
+
+
+(* Apply a function to the expression component of a binding. *)
+Definition mapExpOfBind {T X} 
+  (f: X -> X) (b: @bind X T): @bind X T :=
+ match b with
+ | BBind n t x => BBind n t (f x)
+ end.
+
+
+(********************************************************************)
+(* A substitution is a list of bindings. *)
+Definition subst {X T} := list (@bind X T).
+
+
+(* Apply a function to all the expression components of a list
+   of bindings. *)
+Definition mapExpOfSubst {X T}
+  (f: X -> X) (bs: @subst X T): @subst X T := 
+ map (mapExpOfBind f) bs.
+
+
+(* Lookup the binding with the given name from a substitution. *)
+Fixpoint lookupSubst {X T} 
+   (var: string) (ss: @subst X T): option (@bind X T) :=
+ match ss with
+ |  nil                
+ => None
+
+ |  BBind v t x :: rest
+ => match string_dec var v with 
+    | left _  => Some (BBind v t x)
+    | right _ => lookupSubst var rest
+    end
+ end.
+
+
+(* When we lookup a binding with a particular name from a substitution, 
+   then the returned binding has that name. *)
+Lemma lookupSubst_name 
+ :  forall {X T} n1 n2 t e bs
+ ,  @lookupSubst X T n1 bs = Some (BBind n2 t e)
+ -> n1 = n2.
+Proof.
+ intros.
+ induction bs as [|b].
+ - simpl in *. congruence.
+ - simpl in *. destruct b.
+   remember (string_dec n1 n) as d. destruct d.
+   + inverts H. assumption.
+   + firstorder.
+Qed.
+
+
+(********************************************************************)
+(* Property is true of all pairs of expressions and types in a
+   substitution. *)
+Definition ForallSubstXT {X T} 
+  (P: X -> T -> Prop) (ss: @subst X T): Prop :=
+ Forall2 P (map expOfBind ss) (map typeOfBind ss).
+
+
+(* Fold up a ForallSubstXT *)
+Lemma ForallSubstXT_fold
+ :  forall {X T} (P: X -> T -> Prop) (ss: @subst X T)
+ ,  Forall2 P (map expOfBind ss) (map typeOfBind ss)
+ -> ForallSubstXT P ss.
+Proof.
+ intros.
+ eauto.
+Qed.
+
+
+(* ForallSubstXT append. *)
+Lemma ForallSubstXT_app 
+ :  forall {X T} (P: X -> T -> Prop) ss1 ss2
+ ,  ForallSubstXT P ss1
+ -> ForallSubstXT P ss2
+ -> ForallSubstXT P (ss1 ++ ss2).
+Proof.
+ intros.
+ unfold ForallSubstXT.
+ eapply Forall2_map.
+ eapply Forall2_app.
+ - eapply Forall2_map'; auto.
+ - eapply Forall2_map'; auto.
+Qed.
+
+
+(* Same as Forall2_mp, but keep the definition of
+   ForallSubstXT folded. *)
+Lemma ForallSubstXT_mp
+ :  forall {X T} (P Q: X -> T -> Prop)        ss
+ ,  ForallSubstXT (fun x t => P x t -> Q x t) ss
+ -> ForallSubstXT (fun x t => P x t)          ss
+ -> ForallSubstXT (fun x t => Q x t)          ss.
+Proof.
+ intros.
+ eapply Forall2_mp; eauto.
+Qed.
+
+
+Lemma ForallSubstXT_mapExpOfSubst
+ :  forall {X T} (f: X -> X) (P: X -> T -> Prop) (ss: @subst X T)
+ ,  ForallSubstXT (fun x t => P (f x) t) ss
+ -> ForallSubstXT (fun x t => P x t) (mapExpOfSubst f ss).
+Proof.
+ intros.
+ unfold ForallSubstXT in *.
+ induction ss as [|b].
+ - simpl. auto.
+ - simpl. inverts H.
+   eapply Forall2_cons.
+   + lets D: IHss H5.
+     destruct b.
+     simpl in *. assumption.
+   + eauto. 
+Qed.
+
+
+(********************************************************************)
+(* Strip the expression from a binding, producing a signature. *)
+Fixpoint stripB {X T} (b: @bind X T): @sig T :=
+ match b with
+ | BBind n t _ => SSig n t
+ end.
+
+
+(* Strip a substitution to an environment. *)
+Definition stripS {X T} (ss: @subst X T): @env T :=
+ map stripB ss.
+Hint Transparent stripS.
+
+
+Lemma stripS_fold
+ : forall {X T} ss
+ , map (@stripB X T) ss = stripS ss.
+Proof.
+ eauto.
+Qed.
+
+
+(* Applying a function to the expressions of a substitution,
+   then stripping it yields the same result as just stripping it. *)
+Lemma stripS_mapExpOfSubst
+ : forall {X T} f ss
+ , @stripS X T (mapExpOfSubst f ss) = @stripS X T ss.
+Proof.
+ intros.
+ induction ss as [|b].
+ - simpl. auto.
+ - simpl. rewrite IHss.
+   destruct b. simpl. trivial.
+Qed.
+
+
+Lemma lookup_env_subst_none
+ :  forall {X T} n te ss t
+ ,  @lookupEnv     T n (stripS ss ++ te) = Some t
+ -> @lookupSubst X T n ss                = None
+ -> @lookupEnv     T n te                = Some t.
+Proof.
+ intros.
+ induction ss as [|b].
+ - simpl in *. assumption.
+ - simpl in *. destruct b. simpl in H.
+   remember (string_dec n n0) as d. destruct d.
+   + inverts H. congruence.
+   + eapply IHss. 
+     * auto. 
+     * assumption.
+Qed.
+
+
+Lemma lookup_env_subst_some
+ :  forall {X T} n te ss e t1 t2 P
+ ,  ForallSubstXT  P ss
+ -> @lookupEnv     T n (stripS ss ++ te) = Some t1
+ -> @lookupSubst X T n ss                = Some (BBind n t2 e)
+ -> P e t1.
+Proof.
+ intros. gen n te e t1 t2.
+ induction ss as [|b]; intros.
+ - simpl in *. congruence.
+ - simpl in *. destruct b. simpl in *.
+   remember (string_dec n n0) as d. destruct d.
+   + inverts H0. inverts H1.
+     inverts H. assumption.
+   + inverts H; eauto.
+Qed.
+
